\documentclass[11pt, reqno]{article}
\usepackage{geometry}
\usepackage{amsmath}
\usepackage{amssymb}

\geometry{letterpaper}

\newtheorem{theorem}{Theorem}

\begin{document}


\title{Olympiad Inequalities}
\author{Satvik Saha}
\date{}
\maketitle

\section*{Theorems}

\begin{theorem}[Trivial Inequality]
For all $x \in \mathbb{R}$:
\begin{equation*}
	x^2		\;\geq\;	0
\end{equation*}
\end{theorem}

\begin{theorem}[QM-AM-GM-HM]
For non-negative real numbers $a_1, a_2, \dots, a_n$, the following inequality holds:
\begin{equation*}
	\sqrt{\dfrac{a_1^2 + a_2^2 + \cdots + a_n^2}{n}}	\;\geq\;		\dfrac{a_1 + a_2 + \cdots + a_n}{n}		\;\geq\;
	\sqrt[n]{a_1a_2\cdots a_n}		\;\geq\;		\dfrac{n}{\frac{1}{a_1} + \frac{1}{a_2} + \cdots + \frac{1}{a_n}}
\end{equation*}
Equality holds if and only if $a_1 = a_2 = \cdots = a_n$.
\end{theorem}

\begin{theorem}[Bernoulli]
For all $r \geq 1$ and $x \geq -1$:
\begin{equation*}
	(1 + x)^r	\;\geq\;		1 + xr
\end{equation*}
\end{theorem}

\begin{theorem}[Schur]
Let $a, b, c$ be positive real numbers and $r > 0$. The following inequality holds:
\begin{equation*}
	a^r(a-b)(a-c) + b^r(b-c)(b-a) + c^r(c-a)(c-b)	\;\geq\;		0
\end{equation*}
\end{theorem}

\begin{theorem}[Nesbitt]
Let $a, b, c$ be positive real numbers. The following inequality holds:
\begin{equation*}
	\dfrac{a}{b+c} + \dfrac{b}{c+a} + \dfrac{c}{a+b}		\;\geq\;		\dfrac{3}{2}
\end{equation*}
Equality holds if $a = b = c$.
\end{theorem}

\begin{theorem}[Titu's Lemma]
Let $(a_1, a_2, \dots, a_n)$ and $(b_1, b_2, \dots, b_n)$ be sequences of non-negative real numbers. The following inequality holds:
\begin{equation*}
	\dfrac{a_1^2}{b_1} + \dfrac{a_2^2}{b_2} + \cdots + \dfrac{a_n^2}{b_n}	\;\geq\;		\dfrac{(a_1 + a_2 + \cdots + a_n)^2}{b_1 + b_2 + \cdots + b_n}
\end{equation*}
Equality holds if $\frac{a_1}{b_1} = \frac{a_2}{b_2} = \cdots = \frac{a_n}{b_n}$.
\end{theorem}

\begin{theorem}[Cauchy-Schwarz]
Let $(a_1, a_2, \dots, a_n)$ and $(b_1, b_2, \dots, b_n)$ be sequences of non-negative real numbers. The following inequality holds:
\begin{equation*}
	(a_1^2 + a_2^2 + \cdots + a_n^2)(b_1^2 + b_2^2 + \cdots + b_n^2)	\;\geq\;		(a_1b_1 + a_2b_2 + \cdots + a_nb_n)^2
\end{equation*}
Equality holds if and only if $\frac{a_1}{b_1} = \frac{a_2}{b_2} = \cdots = \frac{a_n}{b_n}$.
\end{theorem}

\begin{theorem}[H\"{o}lder]
Let $(a_1, a_2, \dots, a_n),(b_1, b_2, \dots, b_n),\cdots,(z_1, z_2, \dots, z_n)$ be sequences of non-negative real numbers,
and $\lambda_a, \lambda_b, \cdots, \lambda_z$ be positive reals which sum to $1$. The following inequality holds:
\begin{equation*}
	(a_1 + a_2 + \cdots + a_n)^{\lambda_a} (b_1 + b_2 + \cdots + b_n)^{\lambda_b} \cdots (z_1 + z_2 + \cdots + z_n)^{\lambda_z}	\;\geq\;
	(a_1^{\lambda_a} b_1^{\lambda_b} \!\cdots\! z_1^{\lambda_z} + \;\cdots\; + a_n^{\lambda_a} b_n^{\lambda_b} \!\cdots\! z_n^{\lambda_z})
\end{equation*}
\end{theorem}

\begin{theorem}[Rearrangement]
Let $(a_1 \leq a_2 \leq \cdots \leq a_n)$ and $(b_1 \leq b_2 \leq \cdots \leq b_n)$ be sequences of non-decreasing real numbers.
For any permutation $\pi$ of $\{1, 2, \dots, n\}$, the following inequality holds:
\begin{equation*}
	a_1b_1 + a_2b_2 + \cdots + a_nb_n	\;\geq\;		a_1b_{\pi(1)} + a_2b_{\pi(2)} + \cdots + a_nb_{\pi(n)}	\;\geq\;
	a_1b_n + a_2b_{n-1} + \cdots + a_nb_1
\end{equation*}
\end{theorem}

\begin{theorem}[Chebyshev]
Let $(a_1 \leq a_2 \leq \cdots \leq a_n)$ and $(b_1 \leq b_2 \leq \cdots \leq b_n)$ be sequences of non-decreasing real numbers.
The following inequality holds:
\begin{equation*}
	\dfrac{a_1b_1 + a_2b_2 + \cdots + a_nb_n	}{n} \;\geq\; \dfrac{a_1 + a_2 + \cdots + a_n}{n}\cdot\dfrac{b_1 + b_2 + \cdots + b_n}{n} \;\geq\;
	\dfrac{a_1b_n + a_2b_{n-1} + \cdots + a_nb_1	}{n}
\end{equation*}
\end{theorem}

\begin{theorem}[Muirhead]
Let the sequence $(a_1, a_2, \dots, a_n)$ majorize\footnotemark \, $(b_1, b_2, \dots, b_n)$.
Then, for a sequence of positive reals $(x_1, x_2, \dots, x_n)$, the following inequality holds:
\begin{equation*}
	\sum_{sym}{x_1^{a_1} x_2^{a_2} \cdots x_n^{a_n}}		\;\geq\;		\sum_{sym}{x_1^{b_1} x_2^{b_2} \cdots x_n^{b_n}}	
\end{equation*}
Here, the sums are taken over all permutations of the $n$ variables.
\end{theorem}

\vfill
\footnotetext{
	A sequence $(x_1 \geq x_2 \geq \cdots \geq x_n)$ majorizes $(y_1 \geq y_2 \geq \cdots \geq y_n)$ if
	$\sum{x_i} = \sum{y_i}$ and for all $k = 1, 2, \dots, n-1$
	$$ (x_1 + x_2 + \cdots + x_k) \;\geq\; (y_1 + y_2 + \cdots + y_k)$$
}

\break

\end{document}
