\documentclass[a4paper, 11pt, reqno]{article}

\usepackage[T1]{fontenc}
\usepackage{geometry}
\usepackage{mathtools, amsmath, amssymb}

\geometry{letterpaper}

\title{Telescoping Sums}
\author{Satvik Saha}
\date{}

\newcounter{prob}
\def\problem{\stepcounter{prob}\paragraph{Problem \arabic{prob}}}
\def\solution{\paragraph{Solution}}

\begin{document}
	\maketitle
	
	A sum in which subsequent terms cancel each other, leaving only its initial and final terms is called a
	\textit{telescoping sum}.
	\begin{align*}
		S_n  \; &= \; \sum_{k=0}^{n-1} (T_{k+1} - T_{k})	\\
		     \; &= \; (T_1 - T_0) + (T_2 - T_1) + (T_3 - T_2) + \dots (T_{n} - T_{n-1})	\\
		     \; &= \; T_{n} - T_{0}
	\end{align*}
	
	\problem
	Calculate the given sum.
	\begin{equation*}
		S_n  \; = \;  \frac{1}{1\cdot 2} + \frac{1}{2\cdot 3} + \frac{1}{3\cdot 4} + \dots + \frac{1}{n\cdot (n+1)} 
	\end{equation*}
	\solution
	Define the sequences
	\begin{align*}
		T_k  \; &= \; \frac{1}{k\cdot (k + 1)} \\
		F_k  \; &= \; \frac{1}{k}
	\end{align*}
	Observe that we can write
	\begin{align*}
		T_k 	\; &= \; \frac{(k + 1) - k}{k\cdot (k + 1)}
			\; &= \; \frac{1}{k} - \frac{1}{k + 1}
			\; &= \; F_k - F_{k + 1}
	\end{align*}
	Finally
	\begin{align*}
		\sum_{k=1}^{n} T_k 	\; &= \; \sum_{k=1}^{n} (F_k - F_{k+1})
					\; &= \; F_1 - F_{n + 1}
	\end{align*}
	\begin{equation*}
		\boxed{S_n \; = \;  1 - \frac{1}{n + 1}}
	\end{equation*}
	
	\problem
	Calculate the given sum.
	\begin{equation*}
		S_n \; = \;  \frac{1}{1\cdot 3\cdot 5} + \frac{1}{3\cdot 5\cdot 7} + \frac{1}{5\cdot 7\cdot 9} + \dots + \frac{1}{(2n + 1)(2n + 3)(2n + 5)}
	\end{equation*}
	\solution
	Define the expression for each term and manipulate its factors.
	\begin{align*}
		T_k	\; &= \; \frac{1}{(2k + 1)(2k + 3)(2k + 5)}	\\
			\; &= \; \frac{1}{4(2k + 3)}\left( \frac{1}{2k + 1} - \frac{1}{2k + 5} \right) \\
			\; &= \; \frac{1}{4} \left( \frac{1}{(2k + 1)(2k + 3)} - \frac{1}{(2k + 3)(2k + 5)}\right)	\\
			\; &= \; \frac{1}{8} \left( \frac{1}{2k + 1} - \frac{1}{2k + 3} \right) 
				-\frac{1}{8} \left( \frac{1}{2k + 3} - \frac{1}{2k + 5} \right)
	\end{align*}
	Define the sequence
	\begin{align*}
		F_k	\; &= \; \frac{1}{8 (2k + 1)}	\\
		T_k	\; &= \; (F_k - F_{k + 1}) - (F_{k + 1} - F_{k + 2})	\\
	\end{align*}
	Finally
	\begin{align*}
		\sum_{k=0}^{n} T_k 
			\; &= \; \sum_{k=0}^{n} (F_k - F_{k + 1}) - \sum_{k=0}^{n} (F_{k + 1} - F_{k + 2}) \\
			\; &= \; (F_0 - F_{n + 1}) - (F_1 - F_{n + 2})
	\end{align*}
	\begin{equation*}
		\boxed{ S_n \; = \;  \frac{1}{12} - \frac{1}{4(2n + 3)(2n + 5)} }
	\end{equation*}
	
	\clearpage
	\problem
	Calculate the given sum, to $n$ terms
	\begin{equation*}
		S_n  \;=\;  (1)\cdot 0! \,+\, (3)\cdot 1! \,+\, (7)\cdot 2! \,+\, \dots \,+\, (n^2 - n + 1)\cdot n!
	\end{equation*}
	\solution
	Define the sequences
	\begin{align*}
		T_k  \; &= \;  (k^2 + k + 1)\cdot k! \\
		F_k  \; &= \;  k\cdot k!
	\end{align*}
	Note that $n! = n\cdot (n-1)!$
	\begin{align*}
		F_{k+1}  \; &= \; (k + 1)\cdot (k + 1)! \\
			 \; &= \; (k + 1)\cdot (k + 1)\cdot k! \\
			 \; &= \; (k^2 + 2k + 1)\cdot k! \\
			 \; &= \; (k^2 + k + 1)\cdot k! + k\cdot k! \\
			 \; &= \; T_k + F_k \\
		\Aboxed{T_k \; &= \;  F_{k+1} - F_{k}}
	\end{align*}
	Finally,
	\begin{align*}
		\sum_{k=0}^{n-1} T_k
		 	\; &= \; \sum_{k=0}^{n-1} (F_{k+1} - F_{k}) \\
			\; &= \; F_n - F_0 \\
		\Aboxed{S_n	\; &= \;  n\cdot n!}
	\end{align*}
	
	\clearpage
	\problem
	Calculate the given sum.
	\begin{equation*}
		S_n  \;=\;  \frac{1}{x + 1} + \frac{2}{x^2 + 1} + \frac{4}{x^4 + 1} + \dots + \frac{2^{n-1}}{x^{2^{n-1}} + 1} 
	\end{equation*}
	\solution
	Define the sequences
	\begin{align*}
		T_k \; &= \; \frac{2^k}{x^{2^{k}} + 1} \\
		F_k \; &= \; \frac{2^k}{x^{2^{k}} - 1}
	\end{align*}
	Observe
	\begin{align*}
		F_k - T_k 	\; &= \; 2^k\cdot \left( \frac{1}{x^{2^{k}} - 1} - \frac{1}{x^{2^{k}} + 1} \right) \\
				\; &= \; 2^k\cdot \left( \frac{2}{x^{2^{k}\cdot 2} - 1}  \right) \\
				\; &= \; \frac{2^{k+1}}{x^{2^{k+1}} - 1} \\
				\; &= \; F_{k + 1} \\
		\Aboxed{ T_k \; &= \; F_k - F_{k + 1} }
	\end{align*}
	Finally,
	\begin{align*}
		\sum_{k=0}^{n-1} T_k
		 	\; &= \; \sum_{k=0}^{n-1} (F_{k} - F_{k+1}) \\
			\; &= \; F_0 - F_n \\
		\Aboxed{ S_n	\; &= \; \frac{1}{x - 1} - \frac{2^n}{x^{2^{n}} - 1} }
	\end{align*}
	Note that for $(x > 1)$, L'Hospital's Rule yields
	\begin{align*}
		\lim_{n \to \infty} \left( \frac{2^n}{x^{2^{n}} - 1} \right)
			\; = \;  \lim_{n \to \infty} \left( \frac{2^n\ln{2}}{2^n \ln{2}\cdot x^{2^n}\ln{x}} \right)
			\; = \;  0 
	\end{align*}\\
	\begin{equation*}
		\boxed{ S_\infty \; = \; \frac{1}{x - 1} } \tag{$x > 1$} 
	\end{equation*}

	\problem Define the function $f : \mathbb{N} \to \mathbb{R}$ as follows.
	\begin{equation*}
		f(n) \; = \;  \frac{4n + \sqrt{4n^2 - 1}}{\sqrt{2n+1} + \sqrt{2n-1}} 
	\end{equation*}
	Calculate the sum
	\begin{equation*}
		S_N \; = \; f(1) + f(2) + f(3) + \dots + f(N)
	\end{equation*}
	\solution
	Rationalize and rearrange the expression for $f(n)$ as follows.
	\begin{align*}
		f(n)	\; &= \;  \frac{(4n + \sqrt{2n+1}\sqrt{2n-1})(\sqrt{2n+1} - \sqrt{2n-1})}{(2n + 1) - (2n - 1)} 	\\
			\; &= \;  \frac{1}{2} \left(4n \sqrt{2n+1} - 4n \sqrt{2n-1} + (2n + 1)\sqrt{2n-1} - (2n - 1)\sqrt{2n+1}\right)	\\
			\; &= \;  \frac{1}{2} \left((4n - 2n + 1)\sqrt{2n+1} - (4n - 2n - 1)\sqrt{2n-1}\right) \\
			\; &= \;  \frac{1}{2} \left((2n + 1)^\frac{3}{2} - (2n - 1)^\frac{3}{2}\right)
	\end{align*}
	Define the function $g : \mathbb{N} \to \mathbb{R}$ as follows.
	\begin{align*}
		g(n)	\; &= \;  \frac{1}{2}\cdot (2n + 1)^\frac{3}{2}	\\
		\implies
		g(n - 1)\; &= \;  \frac{1}{2}\cdot (2n - 1)^\frac{3}{2}
	\end{align*}
	Finally
	\begin{align*}
		\sum_{n=1}^{N} f(n) \; &= \;  \sum_{n=1}^{N} \left( g(n) - g(n-1) \right) \\
			\; &= \; g(N) - g(0) 
	\end{align*}
	\begin{equation*}
		\boxed{ S_N \; = \; \frac{1}{2} (2N + 1)^\frac{3}{2} \,-\, \frac{1}{2}}
	\end{equation*}
\end{document}
